theories/compiler.v
@@ -1,0 +1,146 @@
+Require Import refframe.base.
+(* We require functional extensionality such that we can use leibniz
+equiality for compiler_monad. *)
+(* Require Import refframe.axioms. *)
+
+Set Default Proof Using "Type".
+
+Record compiler_monoid := {
+  cm_car :> Type;
+  cm_empty : cm_car;
+  cm_comp : cm_car → cm_car → cm_car;
+  cm_left_id : LeftId (=) cm_empty cm_comp;
+  cm_right_id : RightId (=) cm_empty cm_comp;
+  cm_assoc : Assoc (=) cm_comp;
+}.
+Global Existing Instance cm_left_id.
+Global Existing Instance cm_right_id.
+Global Existing Instance cm_assoc.
+
+Canonical Structure list_compiler_monoid A : compiler_monoid := {|
+  cm_car := list A;
+  cm_empty := [];
+  cm_comp := app;
+|}.
+
+Program Canonical Structure fn_compiler_monoid A : compiler_monoid := {|
+  cm_car := A → A;
+  cm_empty := id;
+  cm_comp := compose;
+|}.
+Next Obligation. done. Qed.
+Next Obligation. done. Qed.
+Next Obligation. done. Qed.
+
+Inductive compiler_success {R E : Type} :=
+| CSuccess (res : R) | CError (err : E).
+Arguments compiler_success : clear implicits.
+
+Record compiler_result {S : Type} {A : compiler_monoid} {E R : Type} := CResult {
+  c_state : S;
+  c_prog : A;
+  c_result : compiler_success R E;
+}.
+Arguments CResult {_ _ _ _}.
+Arguments compiler_result : clear implicits.
+Add Printing Constructor compiler_result.
+
+Definition compiler_monad S A E R : Type := S → compiler_result S A E R.
+
+Global Instance cbind S A E: MBind (compiler_monad S A E) :=
+  λ RA RB f c s,
+    let ra := c s in
+    match ra.(c_result) with
+    | CSuccess r =>
+        let rb := f r ra.(c_state) in
+        CResult rb.(c_state) (cm_comp A ra.(c_prog) rb.(c_prog)) rb.(c_result)
+    | CError e => CResult ra.(c_state) ra.(c_prog) (CError e)
+    end.
+
+Global Instance cret S A E : MRet (compiler_monad S A E) :=
+  λ RA x s, CResult s (cm_empty A) (CSuccess x).
+
+Definition cerror {S A E R} : E → compiler_monad S A E R :=
+  λ err s, CResult s (cm_empty A) (CError err).
+
+Definition cget {S A E} : compiler_monad S A E S :=
+  λ s, CResult s (cm_empty A) (CSuccess s).
+
+Definition cput {S A E} : S → compiler_monad S A E S :=
+  λ s' s, CResult s' (cm_empty A) (CSuccess s).
+
+Definition cappend {S} {A : compiler_monoid} {E} : A → compiler_monad S A E unit :=
+  λ a s, CResult s a (CSuccess tt).
+
+Definition cscope {S A E R} : compiler_monad S A E R → compiler_monad S A E (R * A) :=
+  λ c s,
+    let r := c s in
+    match r.(c_result) with
+    | CSuccess res => CResult r.(c_state) (cm_empty A) (CSuccess (res, r.(c_prog)))
+    | CError err => CResult r.(c_state) (cm_empty A) (CError err)
+    end.
+
+Definition crun {S A E R} : S → compiler_monad S A E R → compiler_result S A E R :=
+  λ s c, c s.
+
+Global Typeclasses Opaque compiler_monad.
+
+Section compiler_monad.
+  Context {S : Type}  {A : compiler_monoid} {E : Type}.
+  Local Notation M := (compiler_monad S A E).
+
+  Lemma run_cbind_cret {RA RB} y (f : RA → M RB) s:
+    crun s (mret y ≫= f) = crun s (f y).
+  Proof. rewrite /crun/mbind/cbind/= left_id_L. by destruct (f y s). Qed.
+
+  Lemma run_cbind_cbind {RA RB RC} x (f : RA → M RB) (g : RB → M RC) s:
+    crun s ((x ≫= f) ≫= g) = crun s (x ≫= λ y, f y ≫= g).
+  Proof.
+    rewrite /crun/mbind/cbind/=.
+    repeat case_match; simplify_eq/= => //.
+    by rewrite assoc_L.
+  Qed.
+
+End compiler_monad.
+
+Module compiler_test.
+
+Local Open Scope Z_scope.
+
+Definition M_test := compiler_monad Z (list_compiler_monoid Z) string.
+
+Definition test_fn : M_test Z :=
+  x ← mret 1;
+  cput x;;
+  y ← cget;
+  cappend [1];;
+  cappend [2];;
+  '(_, z) ← cscope (cappend [3];; cappend [4]);
+  mret (y + sum_list (Z.to_nat <$> z)).
+
+Goal crun 0 test_fn = CResult 1 [1; 2] (CSuccess 8).
+  vm_compute. match goal with | |- ?x = ?x => exact: eq_refl end.
+Abort.
+
+Definition test_error : M_test Z :=
+  x ← cerror "a";
+  cappend [1];;
+  mret x.
+
+Goal crun 0 test_error = CResult 0 [] (CError "a").
+  vm_compute. match goal with | |- ?x = ?x => exact: eq_refl end.
+Abort.
+
+Definition M_test2 := compiler_monad Z (fn_compiler_monoid (list Z)) string.
+
+Definition test_fn2 : M_test2 Z :=
+  x ← mret 1;
+  cappend (λ x, 0::x);;
+  cappend (λ x, 1::x);;
+  mret x.
+
+Goal crun 0 test_fn2 = CResult 0 (λ x : list Z, 0 :: 1 :: x) (CSuccess 1).
+  vm_compute. match goal with | |- ?x = ?x => exact: eq_refl end.
+Abort.
+
+End compiler_test.
